Collectin curret iProps in proof ver.1

theories/HTactics.v
@@ -332,6 +332,54 @@ Section HLEMMAS.
       mk_wf R_src R_tgt ((mr_src, mp_src), (mr_tgt, mp_tgt))
   .
 
+  Variant current_iprops (r: Σ) (I: iProp): Prop :=
+  | current_iprops_intro
+      (GWF: (@URA.wf (GRA.to_URA _) r))
+      (IPROP: Own r ⊢ #=> I)
+  .
+
+  Lemma current_iprops_update I1 r I0
+        (ACC: current_iprops r I0)
+        (UPD: I0 ⊢ #=> I1)
+    :
+      current_iprops r I1.
+  Proof.
+    inv ACC. econs; et.
+    iIntros "H". iApply bupd_trans.
+    iApply UPD. iApply IPROP. iApply "H".
+  Qed.
+
+  (* TODO: find lemma (or typeclass) *)
+  Lemma Upd_Pure P
+    :
+      #=> ⌜P⌝ ⊢ ⌜P⌝.
+  Proof.
+    red. uipropall. i.
+    hexploit (H URA.unit).
+    { rewrite URA.unit_id. et. }
+    i. des. red in H1. red. uipropall.
+  Qed.
+
+  Lemma current_iprops_pure r I P
+        (ACC: current_iprops r I)
+        (PURE: I ⊢ ⌜P⌝)
+    :
+      current_iprops r I /\ <<PURE: P>>.
+  Proof.
+    split; et. inv ACC. hexploit (@to_semantic _ r (⌜P⌝)%I); et.
+    { iIntros "H". iApply Upd_Pure.
+      iApply PURE. iApply IPROP. iApply "H". }
+    i. red in H. uipropall.
+  Qed.
+
+  Lemma current_iprops_exists r A (P: A -> iProp)
+        (ACC: current_iprops r (bi_exist P))
+    :
+      exists x, current_iprops r (P x).
+  Proof.
+    admit "It is not true. Modify HoareCall to make it true".
+  Qed.
+
   Lemma hcall_clo_ord_weaken (o_new: Ord.t)
         Y Z (ftsp1: ftspec Y Z)
         (o: ord) (x: shelve__ ftsp1.(X))
@@ -347,8 +395,8 @@ Section HLEMMAS.
 
         (WEAKER: ftspec_weaker ftsp1 ftsp0)
 
-        (GWF: (@URA.wf (GRA.to_URA _) (URA.add mr_src0 fr_src0)))
-        I (ACC: Own (URA.add mr_src0 fr_src0) ⊢ #=> I)
+        I
+        (ACC: current_iprops (URA.add mr_src0 fr_src0) I)
 
         (UPDATABLE:
            I ⊢ #=> (FR ** R_src a0 mp_src0 ** (ftsp1.(precond) x varg_src varg_tgt o: iProp)))
@@ -361,8 +409,7 @@ Section HLEMMAS.
         (POST: forall (vret_tgt : Any.t) (mr_src1 mr_tgt1 fr_src1: Σ) (mp_src1 mp_tgt1 : Any.t) a1
                       (vret_src: Z)
                       (RTGT: R_tgt a1 mp_tgt1 mr_tgt1)
-                      (GWF: (@URA.wf (GRA.to_URA _) (URA.add mr_src1 fr_src1)))
-                      (ACC: Own (URA.add mr_src1 fr_src1) ⊢ #=> (FR ** R_src a1 mp_src1 ** ftsp1.(postcond) x vret_src vret_tgt))
+                      (ACC: current_iprops (URA.add mr_src1 fr_src1) (FR ** R_src a1 mp_src1 ** ftsp1.(postcond) x vret_src vret_tgt))
           ,
                 gpaco6 (_sim_itree (mk_wf R_src R_tgt)) (cpn6 (_sim_itree (mk_wf R_src R_tgt))) rg rg _ _ eqr o_new
                        (mr_src1, mp_src1, fr_src1, k_src vret_src) (mr_tgt1, mp_tgt1, frs_tgt, k_tgt vret_tgt))
@@ -381,11 +428,11 @@ Section HLEMMAS.
                (<<RSRC: R_src a0 mp_src0 mr_src0'>>) /\
                (<<FRS: FR fr_src0'>>) /\
                (<<PRE: ftsp0.(precond) x_tgt varg_src varg_tgt o rarg_src>>)).
-    { clear - GWF ACC UPDATABLE PRE.
+    { clear - ACC UPDATABLE PRE. inv ACC.
       assert (ENTAIL: Own (mr_src0 ⋅ fr_src0) ⊢ #=> ((FR ** R_src a0 mp_src0) ** (precond ftsp0 x_tgt varg_src varg_tgt o : iProp))).
       { iIntros "H".
         iAssert (#=> ((FR ** R_src a0 mp_src0) ** precond ftsp1 x varg_src varg_tgt o)) with "[H]" as "H".
-        { iApply bupd_trans. iApply UPDATABLE. iApply ACC. iFrame. }
+        { iApply bupd_trans. iApply UPDATABLE. iApply IPROP. iFrame. }
         { iMod "H". iDestruct "H" as "[H0 H1]". iSplitL "H0"; [et|].
           iApply PRE. iApply "H1". }
       }
@@ -419,7 +466,7 @@ Section HLEMMAS.
       { symmetry. eapply OrdArith.add_O_r. }
       { eapply OrdArith.lt_add_r. rewrite Ord.from_nat_S. eapply Ord.S_pos. }
     }
-    i. ired_both; ss. inv WF. eapply POST; et.
+    i. ired_both; ss. inv WF. eapply POST; et. econs; et.
     iStartProof. iIntros "H". iDestruct "H" as "[H0 [H1 H2]]". iSplitR "H2".
     { iSplitL "H1".
       { iApply from_semantic; et. }
@@ -443,8 +490,8 @@ Section HLEMMAS.
 
         (WEAKER: ftspec_weaker ftsp1 ftsp0)
 
-        (GWF: (@URA.wf (GRA.to_URA _) (URA.add mr_src0 fr_src0)))
-        I (ACC: Own (URA.add mr_src0 fr_src0) ⊢ #=> I)
+        I
+        (ACC: current_iprops (URA.add mr_src0 fr_src0) I)
 
         (UPDATABLE:
            I ⊢ #=> (FR ** R_src a0 mp_src0 ** (ftsp1.(precond) x varg_src varg_tgt o: iProp)))
@@ -457,8 +504,7 @@ Section HLEMMAS.
         (POST: forall (vret_tgt : Any.t) (mr_src1 mr_tgt1 fr_src1: Σ) (mp_src1 mp_tgt1 : Any.t) a1
                       (vret_src: Z)
                       (RTGT: R_tgt a1 mp_tgt1 mr_tgt1)
-                      (GWF: (@URA.wf (GRA.to_URA _) (URA.add mr_src1 fr_src1)))
-                      (ACC: Own (URA.add mr_src1 fr_src1) ⊢ #=> (FR ** R_src a1 mp_src1 ** ftsp1.(postcond) x vret_src vret_tgt))
+                      (ACC: current_iprops (URA.add mr_src1 fr_src1) (FR ** R_src a1 mp_src1 ** ftsp1.(postcond) x vret_src vret_tgt))
           ,
                 gpaco6 (_sim_itree (mk_wf R_src R_tgt)) (cpn6 (_sim_itree (mk_wf R_src R_tgt))) rg rg _ _ eqr 100
                        (mr_src1, mp_src1, fr_src1, k_src vret_src) (mr_tgt1, mp_tgt1, frs_tgt, k_tgt vret_tgt))
@@ -485,8 +531,8 @@ Section HLEMMAS.
         (R_src: A -> Any.t -> iProp) (R_tgt: A -> Any.t -> iProp)
         (eqr: Σ * Any.t * Σ -> Σ * Any.t * Σ -> Any.t -> Any.t -> Prop)
 
-        (GWF: (@URA.wf (GRA.to_URA _) (URA.add mr_src0 fr_src0)))
-        I (ACC: Own (URA.add mr_src0 fr_src0) ⊢ #=> I)
+        I
+        (ACC: current_iprops (URA.add mr_src0 fr_src0) I)
 
         (UPDATABLE:
            I ⊢ #=> (FR ** R_src a0 mp_src0 ** (P x varg_src varg_tgt o: iProp)))
@@ -499,8 +545,7 @@ Section HLEMMAS.
         (POST: forall (vret_tgt : Any.t) (mr_src1 mr_tgt1 fr_src1: Σ) (mp_src1 mp_tgt1 : Any.t) a1
                       (vret_src: Z)
                       (RTGT: R_tgt a1 mp_tgt1 mr_tgt1)
-                      (GWF: (@URA.wf (GRA.to_URA _) (URA.add mr_src1 fr_src1)))
-                      (ACC: Own (URA.add mr_src1 fr_src1) ⊢ #=> (FR ** R_src a1 mp_src1 ** Q x vret_src vret_tgt))
+                      (ACC: current_iprops (URA.add mr_src1 fr_src1) (FR ** R_src a1 mp_src1 ** Q x vret_src vret_tgt))
           ,
                 gpaco6 (_sim_itree (mk_wf R_src R_tgt)) (cpn6 (_sim_itree (mk_wf R_src R_tgt))) rg rg _ _ eqr 100
                        (mr_src1, mp_src1, fr_src1, k_src vret_src) (mr_tgt1, mp_tgt1, frs_tgt, k_tgt vret_tgt))
@@ -527,8 +572,7 @@ Section HLEMMAS.
         (ARG:
            forall a x varg_src ord_cur mr_tgt mp_tgt mr_src mp_src fr_src
                   (RTGT: R_tgt a mp_tgt mr_tgt)
-                  (GWF: (@URA.wf (GRA.to_URA _) (URA.add mr_src fr_src)))
-                  (ACC: Own (URA.add mr_src fr_src) ⊢ #=> ((P x varg_src varg_tgt ord_cur: iProp) ** R_src a mp_src)),
+                  (ACC: current_iprops (URA.add mr_src fr_src) ((P x varg_src varg_tgt ord_cur: iProp) ** R_src a mp_src)),
              gpaco6 (_sim_itree (mk_wf R_src R_tgt)) (cpn6 (_sim_itree (mk_wf R_src R_tgt))) rg rg _ _ eqr 90
                     (mr_src, mp_src, fr_src, k_src (x, varg_src, ord_cur))
                     (mr_tgt, mp_tgt, fr_tgt, f_tgt))
@@ -546,7 +590,7 @@ Section HLEMMAS.
     repeat (ired_both; gstep; econs; eauto with ord_step). intro VALID.
     repeat (ired_both; gstep; econs; eauto with ord_step). intro ord_cur.
     repeat (ired_both; gstep; econs; eauto with ord_step). i.
-    ired_both. inv WF. des. eapply ARG; et.
+    ired_both. inv WF. des. eapply ARG; et. econs; et.
     iIntros "H". iDestruct "H" as "[H0 [_ H1]]". iSplitL "H1".
     { iApply from_semantic; et. }
     { iApply from_semantic; et. }
@@ -562,8 +606,8 @@ Section HLEMMAS.
         (eqr: Σ * Any.t * Σ -> Σ * Any.t * Σ -> Any.t -> Any.t -> Prop)
         (FUEL: (14 < n)%ord)
 
-        (GWF: (@URA.wf (GRA.to_URA _) (URA.add mr_src fr_src)))
-        I (ACC: Own (URA.add mr_src fr_src) ⊢ #=> I)
+        I
+        (ACC: current_iprops (URA.add mr_src fr_src) I)
 
         (UPDATABLE:
            I ⊢ #=> (R_src a mp_src ** (Q x vret_src vret_tgt: iProp)))
@@ -584,9 +628,9 @@ Section HLEMMAS.
                (<<UPDATABLE: URA.updatable (URA.add mr_src fr_src) (URA.add mr_src1 rret_src)>>) /\
                (<<RSRC: R_src a mp_src mr_src1>>) /\
                (<<PRE: Q x vret_src vret_tgt rret_src>>)).
-    { clear - GWF ACC UPDATABLE.
+    { clear - ACC UPDATABLE. inv ACC.
       assert (ENTAIL: Own (mr_src ⋅ fr_src) ⊢ #=> (R_src a mp_src ** (Q x vret_src vret_tgt : iProp))).
-      { iIntros "H". iApply bupd_trans. iApply UPDATABLE. iApply ACC. iApply "H". }
+      { iIntros "H". iApply bupd_trans. iApply UPDATABLE. iApply IPROP. iApply "H". }
       eapply to_semantic in ENTAIL; ss.
       clear - GWF ENTAIL. uipropall.
       hexploit (ENTAIL URA.unit).
